With Zoe, Guido: fight a little bit to try to get the bind_wp combinators to type-check, at the cost of a couple admits

examples/refinement/HighComp.fst
@@ -13,17 +13,18 @@ let comp a = state -> M (a * state)
 
 type hwp 'a = state -> ('a * state -> Type) -> Type
 
-// [comp] type with wp 
+// [comp] type with wp
 type comp_wp 'a (wp : hwp 'a) = s0:state -> PURE ('a * state) (wp s0)
 
-let comp_p (a:Type) (pre : state -> Type) (post : state -> a * state -> Type) : GTot Type  = 
+let comp_p (a:Type) (pre : state -> Type) (post : state -> a * state -> Type) : GTot Type  =
     s0:state -> Pure (a * state) (pre s0) (post s0)
 
 // can I get these for free?
-let return_wp (x : 'a) : hwp 'a = fun s0 post -> post (x, s0) 
+let return_wp (x : 'a) : hwp 'a = fun s0 post -> post (x, s0)
 
-let bind_wp (wp1 : state -> ('a * state -> Type) -> Type) 
-            (wp2 : 'a -> state -> ('b * state -> Type) -> Type) : state -> ('b * state -> Type) -> Type = 
+unfold
+let bind_wp (wp1 : state -> ('a * state -> Type) -> Type)
+            (wp2 : 'a -> state -> ('b * state -> Type) -> Type) : state -> ('b * state -> Type) -> Type =
             fun s0 post -> wp1 s0 (function (x, s1) -> wp2 x s1 post)
 
 val hreturn : (a:Type) -> a -> comp a
@@ -33,16 +34,21 @@ val hreturn' : (#a:Type) -> (x:a) -> comp_wp a (return_wp x)
 let hreturn' (#a:Type) (x : a) = fun s -> (x, s)
 
 val hbind : (a:Type) -> (b:Type) -> comp a -> (a -> comp b) -> comp b
-let hbind (a:Type) (b:Type) (m : comp a) (f : a -> comp b) = 
+let hbind (a:Type) (b:Type) (m : comp a) (f : a -> comp b) =
     fun s -> let (a, s1) = m s in f a s1
+
+#set-options "--debug HighComp --debug_level SMTQuery"
 
 let hbind' (#a:Type) (#b:Type) (#wp1:hwp a) (#wp2:a -> hwp b) (m : comp_wp a wp1) (f : (x:a) -> comp_wp b (wp2 x)) :
-  comp_wp b (bind_wp wp1 wp2) = 
-    fun s -> let (a, s1) = m s in f a s1
+  comp_wp b (bind_wp wp1 wp2) =
+  fun s ->
+    admit ();
+    let (a, s1) = m s in
+    f a s1
 
 val hread : i:int -> comp mint
-let hread (i:int) : comp mint = 
-    fun s -> if i = 0 then (fst s, s) 
+let hread (i:int) : comp mint =
+    fun s -> if i = 0 then (fst s, s)
           else (snd s, s)
 
 val hwrite : i:int -> v:mint -> comp unit
@@ -54,18 +60,18 @@ let write_wp (i:nat) (v:mint) : hwp unit = fun s0 post -> post (hwrite i v s0)
 
 let read_wp (i:nat) : hwp mint = fun s0 post -> post (hread i s0)
 
-val hread' : i:int -> comp_wp mint (read_wp i)
-let hread' (i:int) : comp_wp mint (read_wp i) = 
-    fun s -> if i = 0 then (fst s, s) 
+val hread' : i:nat -> comp_wp mint (read_wp i)
+let hread' (i:nat) : comp_wp mint (read_wp i) =
+    fun s -> if i = 0 then (fst s, s)
           else (snd s, s)
 
-val hwrite' : i:int -> v:mint -> comp_wp unit (write_wp i v)
-let hwrite' (i:int) (v:mint) : comp_wp unit (write_wp i v) =
+val hwrite' : i:nat -> v:mint -> comp_wp unit (write_wp i v)
+let hwrite' (i:nat) (v:mint) : comp_wp unit (write_wp i v) =
     fun s -> if i = 0 then ((), (v, snd s))
           else ((), (fst s, v))
 
 val dread : unit -> comp state
-let dread (_ : unit) : comp state = fun s -> (s, s) 
+let dread (_ : unit) : comp state = fun s -> (s, s)
 
 val dwrite : v:state -> comp unit
 let dwrite (v : state) : comp unit = fun s -> ((), v)
@@ -75,7 +81,7 @@ let dwrite (v : state) : comp unit = fun s -> ((), v)
 
 total reifiable reflectable new_effect {
       HIGH : a:Type -> Effect
-      with repr  = comp 
+      with repr  = comp
        ; bind     = hbind
        ; return   = hreturn
        ; get      = hread
